Updates

generic/Zeta.Generic.Interleave.fst
@@ -57,3 +57,12 @@ let thread_state_pre (#vspec: verifier_spec) (#n:_) (tid:nat{tid < n})
 let thread_state_post (#vspec: verifier_spec) (#n:_) (tid:nat{tid < n})
   : IF.idxfn_t (gen_seq vspec n) (v:vspec.vtls_t {vspec.valid v})
   = admit()
+
+let lemma_add_evict_set_identical_glog_aux (#vspec #n:_) (ep: epoch) (il: verifiable_log vspec n)
+  : Lemma (ensures (add_set ep il == G.add_set ep (to_glog il) /\
+                    evict_set ep il == G.evict_set ep (to_glog il)))
+  = admit()
+
+let lemma_add_evict_set_identical_glog (#vspec #n:_) (epmax: epoch) (il: verifiable_log vspec n)
+  : Lemma (ensures (aems_equal_upto epmax il <==> G.aems_equal_upto epmax (to_glog il)))
+  = admit()
