high2/Zeta.High.Verifier.EAC.fsti
@@ -1,13 +1,16 @@
 module Zeta.High.Verifier.EAC
 
 open Zeta.Time
+open Zeta.HashCollision
 open Zeta.EAC
+open Zeta.Generic.Interleave
 open Zeta.High.Verifier
 open Zeta.High.TSLog
 
-(*
+module GI = Zeta.Generic.Interleave
+
 val lemma_neac_implies_hash_collision
-  (#app:_)
+  (#app #n:_)
   (epmax: epoch)
-  (itsl: neac_before_epoch epmax )
-*)
+  (itsl: neac_before_epoch app n epmax {GI.aems_equal_upto epmax itsl})
+  : hash_collision app
